theories/Crypt/package/pkg_semantics.v
@@ -41,7 +41,7 @@ Arguments ropr {_ _ _} _ _.
 
 *)
 Fixpoint repr {A : choiceType} (p : raw_code A) :
-  rFreeF (@ops_StP heap_choiceType) (@ar_StP heap_choiceType) A :=
+  rFreeF (@ops_StP heap) (@ar_StP heap) A :=
   match p with
   | ret x => retrFree x
   | opr o x k =>
@@ -74,7 +74,7 @@ Proof.
 Qed.
 
 Definition repr_cmd {A} (c : command A) :
-  rFreeF (@ops_StP heap_choiceType) (@ar_StP heap_choiceType) A :=
+  rFreeF (@ops_StP heap) (@ar_StP heap) A :=
   match c with
   | cmd_op o x => retrFree (chCanonical (chtgt o))
   | cmd_get ℓ =>
